implementing get using reflect

ulib/Steel.RST.fst
@@ -214,39 +214,65 @@ let subcomp a r_in r_out wp_f wp_g f = f
 
 let lift_div_rstate a wp r f = fun _ -> f ()
 
+
+/// Implementation of the `get` action
+///
+/// We implement `get` by using reflect
+///
+/// For better F* type inference, we do it in two steps:
+///   -- first define the underlying STATE function, with a `repr` type
+///      annotating an explicit `repr` type helps F* type inference
+///   -- and then reflect it into the desired type
+///
+/// `get_` is the underlying STATE function with a `repr` type
+
+let get_ (r:resource)
+: repr (rmem r) r (fun _ -> r) (fun p h -> p h h)
+= fun _ ->
+  let h = HST.get () in
+  mk_rmem r h
+
+let get r = RST?.reflect (get_ r)
+
 open Steel.Tactics
 
 #set-options "--z3rlimit 20"
 
-let st_wp_monotonic (a: Type) (wp: st_wp a) =
-  forall (p q: st_post a). (forall x h. p x h ==> q x h) ==> (forall h . wp p h ==> wp q h)
+/// With latest layered effects branch, F* will not allow the lift from STATE to RSTATE
+///
+/// To move between a layered effect and its underlying effect, use `reify` and `reflect`
 
-let lift_state_rstate
-  (a:Type)
-  (r_in:resource)
-  (r_out:a -> resource)
-  (wp_st: st_wp a{st_wp_monotonic a wp_st})
-  (f: unit -> STATE a wp_st)
-  : repr a r_in r_out (fun (post: r_post a r_out) -> (
-    fun (h_in: rmem r_in) -> (forall (h0: imem (inv r_in){h_in == mk_rmem r_in h0}).
-      inv r_in h0 /\ rst_inv r_in h0 /\
-      wp_st (fun (x:a) (h1: HS.mem) ->
-        inv (r_out x) h1 /\
-        rst_inv (r_out x) h1 /\
-        modifies r_in (r_out x) h0 h1 /\
-	post x (mk_rmem (r_out x) h1)
-      ) h0
-    ))
-  )
-  =
-  fun _ -> f ()
+// let st_wp_monotonic (a: Type) (wp: st_wp a) =
+//   forall (p q: st_post a). (forall x h. p x h ==> q x h) ==> (forall h . wp p h ==> wp q h)
 
-sub_effect STATE ~> RSTATE = lift_state_rstate
+// let lift_state_rstate
+//   (a:Type)
+//   (r_in:resource)
+//   (r_out:a -> resource)
+//   (wp_st: st_wp a{st_wp_monotonic a wp_st})
+//   (f: unit -> STATE a wp_st)
+//   : repr a r_in r_out (fun (post: r_post a r_out) -> (
+//     fun (h_in: rmem r_in) -> (forall (h0: imem (inv r_in){h_in == mk_rmem r_in h0}).
+//       inv r_in h0 /\ rst_inv r_in h0 /\
+//       wp_st (fun (x:a) (h1: HS.mem) ->
+//         inv (r_out x) h1 /\
+//         rst_inv (r_out x) h1 /\
+//         modifies r_in (r_out x) h0 h1 /\
+// 	post x (mk_rmem (r_out x) h1)
+//       ) h0
+//     ))
+//   )
+//   =
+//   fun _ -> f ()
 
-let get r =
-  let h = HST.get () in
-  mk_rmem r h
+// sub_effect STATE ~> RSTATE = lift_state_rstate
 
+// let get r =
+//   let h = HST.get () in
+//   mk_rmem r h
+
+
+/// Implement `rst_frame` as an action using reflect the same way we did for `get`
 
 #push-options "--no_tactics --z3rlimit 100 --max_fuel 0 --max_ifuel 0"
 
